injectivity of pi, computation for cast, no confusion

theories/SetModel/HO_obseq.v
@@ -1,6 +1,6 @@
 Require Import library.
 Require Import ZF_axioms ZF_library ZF_nat.
-Require Import HO HO_prop HO_univ HO_forall HO_pi.
+Require Import HO HO_prop HO_univ HO_forall HO_nat HO_pi.
 
 (* Observational equality *)
 
@@ -100,7 +100,93 @@ Proof.
   - unfold implTy_HO in He. specialize (He γ Hγ). apply ZFincomp in He. now destruct He.
   - unfold implTy_HO in Hf. specialize (Hf γ Hγ). apply ZFincomp in Hf. now destruct Hf.
 Qed.
-  
+
 (* Injectivity of Pi-types *)
 
-(* Computation rules for cast *)
+Definition piinj1Tm_HO (A A' B B' e : ZFSet -> ZFSet) : ZFSet -> ZFSet := fun _ => ∅.
+
+Lemma piinj1Tm_HO_typing {n : nat} {Γ : ZFSet} {A A' B B' e : ZFSet -> ZFSet}
+  (HA : ∀ γ ∈ Γ, A γ ∈ 𝕌 n) (HB : ∀ γa ∈ ctxExt n Γ A, B γa ∈ 𝕌 n)
+  (HA' : ∀ γ ∈ Γ, A' γ ∈ 𝕌 n) (HB' : ∀ γa ∈ ctxExt n Γ A', B' γa ∈ 𝕌 n)
+  (He : ∀ γ ∈ Γ, e γ ∈ eqTy_HO (univTy_HO n) (piTy_HO n A B) (piTy_HO n A' B') γ)
+  : ∀ γ ∈ Γ, piinj1Tm_HO A A' B B' e γ ∈ eqTy_HO (univTy_HO n) A' A γ.
+Proof.
+  intros γ Hγ. cbn. unfold eqTy_HO. unfold piinj1Tm_HO. apply prop_true_iff. apply sym.
+  apply (piTy_HO_inj1 HA HB HA' HB' Hγ). specialize (He γ Hγ). unfold eqTy_HO in He.
+  now apply prop_true_if in He.
+Qed.
+
+Definition piinj2Tm_HO (A A' B B' e a : ZFSet -> ZFSet) : ZFSet -> ZFSet := fun _ => ∅.
+
+Lemma piinj2Tm_HO_typing {n : nat} {Γ : ZFSet} {A A' B B' e a : ZFSet -> ZFSet}
+  (HA : ∀ γ ∈ Γ, A γ ∈ 𝕌 n) (HB : ∀ γa ∈ ctxExt n Γ A, B γa ∈ 𝕌 n)
+  (HA' : ∀ γ ∈ Γ, A' γ ∈ 𝕌 n) (HB' : ∀ γa ∈ ctxExt n Γ A', B' γa ∈ 𝕌 n)
+  (He : ∀ γ ∈ Γ, e γ ∈ eqTy_HO (univTy_HO n) (piTy_HO n A B) (piTy_HO n A' B') γ)
+  (Ha : ∀ γ ∈ Γ, a γ ∈ 𝕌el n (A' γ)) (a0 := castTm_HO A' A (piinj1Tm_HO A A' B B' e) a)
+  : ∀ γ ∈ Γ, piinj2Tm_HO A A' B B' e a γ ∈ eqTy_HO (univTy_HO n) (fun γ => B ⟨ γ ; a0 γ ⟩) (fun γ => B' ⟨ γ ; a γ ⟩) γ.
+Proof.
+  intros γ Hγ. cbn. unfold piinj2Tm_HO. unfold eqTy_HO. apply prop_true_iff.
+  unfold castTm_HO in a0. unfold a0. clear a0. specialize (He γ Hγ). unfold eqTy_HO in He.
+  apply prop_true_if in He. assert (a γ ∈ 𝕌el n (A γ)).
+  { refine (transpS (fun X => a γ ∈ 𝕌el n X) _ (Ha γ Hγ)). apply sym.
+    now apply (piTy_HO_inj1 HA HB HA' HB' Hγ). }
+  apply (piTy_HO_inj2 HA HB HA' HB' Hγ He H).
+Qed.
+
+(* Computation rule for cast on pi
+   Since cast is the identity, this rule is just η, modulo a bit of transport *)
+
+Lemma castTm_HO_pi {n : nat} {Γ : ZFSet} {A A' B B' e f : ZFSet -> ZFSet}
+  (HA : ∀ γ ∈ Γ, A γ ∈ 𝕌 n) (HB : ∀ γa ∈ ctxExt n Γ A, B γa ∈ 𝕌 n)
+  (HA' : ∀ γ ∈ Γ, A' γ ∈ 𝕌 n) (HB' : ∀ γa ∈ ctxExt n Γ A', B' γa ∈ 𝕌 n)
+  (He : ∀ γ ∈ Γ, e γ ∈ eqTy_HO (univTy_HO n) (piTy_HO n A B) (piTy_HO n A' B') γ)
+  (Hf : ∀ γ ∈ Γ, f γ ∈ 𝕌el n (piTy_HO n A B γ))
+  (Au := fun γa => A (ctx_wk n Γ A' γa)) (A'u := fun γa => A' (ctx_wk n Γ A' γa))
+  (Bu := fun γaa => B ⟨ ctx_wk n Γ A' (ctx_wk n (ctxExt n Γ A') Au γaa) ; ctx_var0 n (ctxExt n Γ A') Au γaa ⟩)
+  (B'u := fun γaa => B' ⟨ ctx_wk n Γ A' (ctx_wk n (ctxExt n Γ A') A'u γaa) ; ctx_var0 n (ctxExt n Γ A') A'u γaa ⟩)
+  (t1 := castTm_HO A'u Au (piinj1Tm_HO Au A'u Bu B'u (fun γa => e (ctx_wk n Γ A' γa))) (fun γa => ctx_var0 n Γ A' γa))
+  (t2 := appTm_HO n Au (fun γa => f (ctx_wk n Γ A' γa)) t1)
+  (t3 := castTm_HO (fun γa => B ⟨ ctx_wk n Γ A' γa ; t1 γa ⟩) B'
+           (piinj2Tm_HO Au A'u Bu B'u (fun γa => e (ctx_wk n Γ A' γa)) (fun γa => ctx_var0 n Γ A' γa)) t2)
+  (t4 := lamTm_HO n A' t3) : ∀ γ ∈ Γ, castTm_HO (piTy_HO n A B) (piTy_HO n A' B') e f γ ≡ t4 γ.
+Proof.
+  intros γ Hγ. unfold castTm_HO in *. unfold t4. unfold t3. unfold t2. unfold t1. unfold Au.
+  clear t1 t2 t3 t4. unfold lamTm_HO. unfold appTm_HO.
+  specialize (He γ Hγ). unfold eqTy_HO in He. apply prop_true_if in He.
+  assert (A γ ≡ A' γ) as HAA'. { now apply (piTy_HO_inj1 HA HB HA' HB' Hγ). }
+  assert (f γ ∈ setPi n (𝕌el n (A' γ)) (fun a => 𝕌el n (B' ⟨ γ ; a ⟩))) as Hf'.
+  { refine (transpS (fun X => f γ ∈ X) (el_piTy HA' HB' Hγ) _).
+    refine (transpS (fun X => f γ ∈ 𝕌el n X) He _). now apply Hf. }
+  apply ZFincomp in Hf'. destruct Hf' as [ Hf' _ ].
+  apply (setArr_funext (A := 𝕌el n (A' γ)) (B := 𝕍 n)).
+  - exact Hf'.
+  - apply relToGraph_typing. apply HO_rel_typing. intros a Ha.
+    refine (transp2S (fun X Y => setAppArr (𝕌el n (A X)) (𝕍 n) (f X) Y ∈ 𝕍 n)
+              (sym (ctxExtβ1 HA' Hγ Ha)) (sym (ctxExtβ2 HA' Hγ Ha)) _).
+    refine (transpS (fun X => setAppArr (𝕌el n X) (𝕍 n) (f γ) a ∈ 𝕍 n) (sym HAA') _).
+    apply setAppArr_typing. 2:assumption. exact Hf'.
+  - intros a Ha. refine (sym _). refine (trans _ _). apply setAppArr_HO. 2:assumption.
+    + clear a Ha. intros a Ha. 
+      refine (transp2S (fun X Y => setAppArr (𝕌el n (A X)) (𝕍 n) (f X) Y ∈ 𝕍 n)
+                (sym (ctxExtβ1 HA' Hγ Ha)) (sym (ctxExtβ2 HA' Hγ Ha)) _).
+      refine (transpS (fun X => setAppArr (𝕌el n X) (𝕍 n) (f γ) a ∈ 𝕍 n) (sym HAA') _).
+      apply setAppArr_typing. 2:assumption. exact Hf'.
+    + refine (fequal2 (fun X Y => setAppArr (𝕌el n (A X)) (𝕍 n) (f X) Y)
+                ((ctxExtβ1 HA' Hγ Ha)) ((ctxExtβ2 HA' Hγ Ha))).
+Qed.
+
+(* No-confusion theorems. Copy and paste for all type formers if necessary *)
+
+Lemma nat_neq_pi {n : nat} {Γ : ZFSet} {A B e : ZFSet -> ZFSet}
+  (HA : ∀ γ ∈ ⋆, A γ ∈ 𝕌 n) (HB : ∀ γa ∈ ctxExt n ⋆ A, B γa ∈ 𝕌 n)
+  (He : ∀ γ ∈ ⋆, e γ ∈ eqTy_HO (univTy_HO n) natTy_HO (piTy_HO n A B) γ) : FalseS.
+Proof.
+  assert (∅ ∈ ⋆) as H. { now apply inSetSingl. }
+  specialize (He _ H). cbn in He. unfold eqTy_HO in He. apply prop_true_if in He.
+  assert (ZFzero ≡ ZFone).
+  { refine (trans (sym _) (trans (fequal (𝕌hd n) He) _)).
+    - now apply hd_natTy.
+    - now apply (hd_piTy HA HB H). }
+  now apply (zero_ne_suc ∅).
+Qed.
+
